Remove most of stateT from Basics.v. Need to figure out Events/State.v resolution issue

theories/Basics/Basics.v
@@ -51,15 +51,6 @@ Module Monads.
 
 Definition identity (a : Type) : Type := a.
 
-Definition stateT (s : Type) (m : Type -> Type) (a : Type) : Type :=
-  s -> m (prod s a).
-Definition state (s a : Type) := s -> prod s a.
-
-Definition run_stateT {s m a} (x : stateT s m a) : s -> m (s * a)%type := x.
-
-Definition liftState {s a f} `{Functor f} (fa : f a) : Monads.stateT s f a :=
-  fun s => pair s <$> fa.
-
 Definition readerT (r : Type) (m : Type -> Type) (a : Type) : Type :=
   r -> m a.
 Definition reader (r a : Type) := r -> a.
@@ -67,19 +58,6 @@ Definition reader (r a : Type) := r -> a.
 Definition writerT (w : Type) (m : Type -> Type) (a : Type) : Type :=
   m (prod w a).
 Definition writer := prod.
-
-#[global] Instance Functor_stateT {m s} {Fm : Functor m} : Functor (stateT s m)
-  := {|
-    fmap _ _ f := fun run s => fmap (fun sa => (fst sa, f (snd sa))) (run s)
-    |}.
-
-#[global] Instance Monad_stateT {m s} {Fm : Monad m} : Monad (stateT s m)
-  := {|
-    ret _ a := fun s => ret (s, a)
-  ; bind _ _ t k := fun s =>
-      sa <- t s ;;
-      k (snd sa) (fst sa)
-    |}.
 
 End Monads.
 
@@ -110,18 +88,6 @@ Polymorphic Class MonadIter (M : Type -> Type) : Type :=
           | inl i' => inl (i', snd is')
           | inr r => inr (r, snd is')
           end) (i, s)).
-
-#[global] Polymorphic Instance MonadIter_stateT0 {M S} {MM : Monad M} {AM : MonadIter M}
-  : MonadIter (Monads.stateT S M) :=
-  fun _ _ step i s =>
-    iter (fun si =>
-      let s := fst si in
-      let i := snd si in
-      si' <- step i s;;
-      ret match snd si' with
-          | inl i' => inl (fst si', i')
-          | inr r => inr (fst si', r)
-          end) (s, i).
 
 #[global] Instance MonadIter_readerT {M S} {AM : MonadIter M} : MonadIter (readerT S M) :=
   fun _ _ step i => mkReaderT (fun s =>
