theories/Basics/MonadState.v
@@ -4,16 +4,18 @@ From Coq Require Import
      Morphisms.
 
 From ExtLib Require Import
-     Structures.Monad.
-
+  Structures.Monad
+  Structures.MonadState
+  Data.Monads.StateMonad.
+  
 From ITree Require Import
      Basics.Basics
      Basics.Category
+     Basics.CategoryTheory
      Basics.CategoryKleisli
      Basics.CategoryKleisliFacts
      Basics.Monad.
 
-Import ITree.Basics.Basics.Monads.
 Import CatNotations.
 Local Open Scope cat_scope.
 Local Open Scope cat.
@@ -26,10 +28,11 @@ Section State.
   Context {HEQP: @Eq1Equivalence M _ EQM}.
   Context {ML: @MonadLawsE M _ HM}.
 
-  Global Instance Eq1_stateTM : Eq1 (stateT S M).
-  Proof.
-    exact (fun a => pointwise_relation _ eq1).
-  Defined.
+  (* Re-export Monad_stateT from ExtLib *)
+  Global Existing Instance Monad_stateT.
+  
+  Global Instance Eq1_stateTM : Eq1 (stateT S M) :=
+    fun _ a b => forall s, eq1 (runStateT a s) (runStateT b s).
 
   Global Instance Eq1Equivalence_stateTM : @Eq1Equivalence (stateT S M) _ Eq1_stateTM.
   Proof.
@@ -44,20 +47,24 @@ Section State.
   Proof.
   constructor.
   - cbn. intros a b f x.
-    repeat red.  intros s.
+    repeat red.  intros s. cbn.
     rewrite bind_ret_l. reflexivity.
   - cbn. intros a x.
-    repeat red. intros s.
-    assert (EQM _ (bind (x s) (fun sa : S * a => ret (fst sa, snd sa))) (bind (x s) (fun sa => ret sa))).
-    { apply Proper_bind. reflexivity. intros.  repeat red. destruct a0; reflexivity. }
-    rewrite H.
-    rewrite bind_ret_r. reflexivity.
+    repeat red. intros s. cbn.
+    cut (EQM _
+              (bind (runStateT x s) (fun sa : a * S => let (v, s0) := sa in ret (v, s0)))
+              (bind (runStateT x s) (fun sa => ret sa))).
+    + intro HeqM.
+      rewrite bind_ret_r in HeqM.
+      apply HeqM.
+    + apply Proper_bind. reflexivity. intros.  repeat red. destruct a0; reflexivity. 
   - cbn. intros a b c x f g.
     repeat red. intros s.
+    cbn.
     rewrite bind_bind.
     apply Proper_bind.
     + reflexivity.
-    + reflexivity.
+    + unfold pointwise_relation; intros (? & ?); reflexivity.
   - repeat red. intros a b x y H x0 y0 H0 s.
     apply Proper_bind.
     + apply H.
@@ -69,20 +76,20 @@ Section State.
   Context {IM: Iter (Kleisli M) sum}.
   Context {CM: Iterative (Kleisli M) sum}.
 
-  Definition iso {a b:Type} (sab : S * (a + b)) : (S * a) + (S * b) :=
-    match sab with
-    | (s, inl x) => inl (s, x)
-    | (s, inr y) => inr (s, y)
+  Definition iso {a b:Type} (sab : (a + b) * S) : (a * S) + (b * S) :=
+    match sab with 
+    | (inl x, s) => inl (x, s)
+    | (inr y, s) => inr (y, s)
     end.
 
-  Definition iso_inv {a b:Type} (sab : (S * a) + (S * b)) : S * (a + b) :=
+  Definition iso_inv {a b:Type} (sab : (a * S) + (b * S)) : (a + b) * S :=
     match sab with
-    | inl (s, a) => (s, inl a)
-    | inr (s, b) => (s, inr b)
+    | inl (a, s) => (inl a, s)
+    | inr (b, s) => (inr b, s)
     end.
 
-  Definition internalize {a b:Type} (f : Kleisli (stateT S M) a b) : Kleisli M (S * a) (S * b) :=
-    fun (sa : S * a) => f (snd sa) (fst sa).
+  Definition internalize {a b:Type} (f : Kleisli (stateT S M) a b) : Kleisli M (a * S) (b * S) :=
+    fun (sa : a * S) => runStateT (f (fst sa)) (snd sa).
 
   Lemma internalize_eq {a b:Type} (f g : Kleisli (stateT S M) a b) :
     eq2 f g <-> eq2 (internalize f) (internalize g).
@@ -94,10 +101,9 @@ Section State.
     - intros.
       repeat red. intros.
       unfold internalize in H.
-      specialize (H (a1, a0)).
+      specialize (H (a0, s)).
       apply H.
   Qed.
-
 
   Lemma internalize_cat {a b c} (f : Kleisli (stateT S M) a b) (g : Kleisli (stateT S M) b c) :
     (internalize (f >>> g)) ⩯ ((internalize f) >>> (internalize g)).
@@ -108,12 +114,12 @@ Section State.
     unfold internalize.
     unfold cat, Cat_Kleisli.
     cbn.
-    reflexivity.
+    apply Proper_bind; try reflexivity.
+    unfold pointwise_relation; intros (? & ?); reflexivity.
   Qed.
 
-
-  Lemma internalize_pure {a b c} (f : Kleisli (stateT S M) a b) (g : S * b -> S * c) :
-    internalize f >>> pure g   ⩯   (internalize (f >>> (fun b s => ret (g (s,b))))).
+  Lemma internalize_pure {a b c} (f : Kleisli (stateT S M) a b) (g : b * S -> c * S) :
+    internalize f >>> pure g ⩯ (internalize (f >>> (fun b => mkStateT (fun s => ret (g (b,s)))))).
   Proof.
     repeat red.
     destruct a0.
@@ -125,13 +131,9 @@ Section State.
       unfold pure. reflexivity.
   Qed.
 
-
-  Global Instance Iter_stateTM : Iter (Kleisli (stateT S M)) sum.
-  Proof.
-    exact
-      (fun (a b : Type) (f : a -> S -> M (S * (a + b))) (x:a) (s:S) =>
-        iter ((internalize f) >>> (pure iso)) (s, x)).
-  Defined.
+  Global Instance Iter_stateTM : Iter (Kleisli (stateT S M)) sum :=
+    fun _ _ f a =>
+      mkStateT (fun s => iter ((internalize f) >>> (pure iso)) (a, s)).
 
   Global Instance Proper_Iter_stateTM : forall a b, @Proper (Kleisli (stateT S M) a (a + b) -> (Kleisli (stateT S M) a b)) (eq2 ==> eq2) iter.
   Proof.
@@ -144,29 +146,29 @@ Section State.
     cbn.
     apply Proper_bind.
     - apply H.
-    - repeat red. destruct a2 as [s' [x1|y1]]; reflexivity.
+    - repeat red. destruct a2 as [[x1|y1] s']; reflexivity.
  Qed.
 
   Global Instance IterUnfold_stateTM : IterUnfold (Kleisli (stateT S M)) sum.
   Proof.
-  destruct CM.
-  unfold IterUnfold.
-  intros a b f.
-  repeat red.
-  intros a0 s.
-  unfold cat, Cat_Kleisli.
-  unfold iter, Iter_stateTM.
-  rewrite iterative_unfold.  (* SAZ: why isn't iter_unfold exposed here? *)
-  unfold cat, Cat_Kleisli.
-  simpl.
-  rewrite bind_bind.
-  apply Proper_bind.
-  + reflexivity.
-  + repeat red. destruct a1 as [s' [x | y]]; simpl.
-    * unfold pure. rewrite bind_ret_l.
-      reflexivity.
-    * unfold pure. rewrite bind_ret_l.
-      reflexivity.
+    destruct CM.
+    unfold IterUnfold.
+    intros a b f.
+    repeat red.
+    intros a0 s.
+    unfold cat, Cat_Kleisli.
+    unfold iter, Iter_stateTM.
+    cbn.
+    rewrite iterative_unfold.  (* SAZ: why isn't iter_unfold exposed here? *)
+    unfold cat, Cat_Kleisli.
+    rewrite bind_bind.
+    apply Proper_bind.
+    + reflexivity.
+    + repeat red. destruct a1 as [[x | y] s']; simpl.
+      * unfold pure. rewrite bind_ret_l.
+        reflexivity.
+      * unfold pure. rewrite bind_ret_l.
+        reflexivity.
   Qed.
 
   Global Instance IterNatural_stateTM : IterNatural (Kleisli (stateT S M)) sum.
@@ -185,7 +187,7 @@ Section State.
     rewrite! bind_bind.
     apply Proper_bind.
     - reflexivity.
-    - repeat red. destruct a2 as [s' [x | y]]; simpl.
+    - repeat red. destruct a2 as [[x | y] s']; simpl.
       + unfold pure. rewrite bind_ret_l.
         cbn. unfold cat, Cat_Kleisli. cbn.
         rewrite bind_bind.
@@ -204,20 +206,18 @@ Section State.
   Qed.
 
   Lemma internalize_pure_iso {a b c} (f : Kleisli (stateT S M) a (b + c)) :
-    ((internalize f) >>> pure iso) ⩯ (fun sa => (bind (f (snd sa) (fst sa))) (fun sbc => ret (iso sbc))).
+    ((internalize f) >>> pure iso) ⩯ (fun sa => (bind (runStateT (f (fst sa)) (snd sa))) (fun sbc => ret (iso sbc))).
   Proof.
     reflexivity.
   Qed.
 
-
   Lemma eq2_to_eq1 : forall a b (f g : Kleisli (stateT S M) a b) (x:a) (s:S),
       eq2 f g ->
-      eq1 (f x s) (g x s).
+      eq1 (runStateT (f x) s) (runStateT (g x) s).
   Proof.
     intros a b f g x s H.
     apply H.
   Qed.
-
 
   Lemma iter_dinatural_helper:
     forall (a b c : Type) (f : Kleisli (stateT S M) a (b + c)) (g : Kleisli (stateT S M) b (a + c)),
@@ -233,7 +233,7 @@ Section State.
     apply Proper_bind.
     - reflexivity.
     - repeat red.
-      destruct a1 as [s' [x | y]].
+      destruct a1 as [[x | y] s'].
       + unfold pure.
         rewrite bind_ret_l.
         unfold case_, Case_Kleisli, Function.case_sum.
@@ -243,7 +243,6 @@ Section State.
           cbn.
           rewrite bind_ret_l. reflexivity.
   Qed.
-
 
   Global Instance IterDinatural_stateTM : IterDinatural (Kleisli (stateT S M)) sum.
   Proof.
@@ -263,7 +262,7 @@ Section State.
     apply Proper_bind.
     - reflexivity.
     - repeat red.
-      destruct a2 as [s [x | y]].
+      destruct a2 as [[x | y] s].
       + unfold pure.
         rewrite bind_ret_l.
         cbn.
@@ -274,7 +273,7 @@ Section State.
         apply Proper_bind.
         * reflexivity.
         * repeat red.
-          destruct a2 as [s' [x' | y]].
+          destruct a2 as [[x' | y] s'].
           ** cbn.  rewrite bind_ret_l. unfold case_, Case_Kleisli, Function.case_sum.
              reflexivity.
           ** cbn.  rewrite bind_ret_l. unfold case_, Case_Kleisli, Function.case_sum.
@@ -283,9 +282,8 @@ Section State.
         rewrite bind_ret_l.
         cbn.
         reflexivity.
-    Qed.
-
-
+  Qed.
+  
   Global Instance IterCodiagonal_stateTM : IterCodiagonal (Kleisli (stateT S M)) sum.
   Proof.
     destruct CM.
@@ -298,13 +296,13 @@ Section State.
     eapply iterative_proper_iter.
     eapply Proper_cat_Kleisli.
 
-    assert (internalize (fun (x:a) (s:S) => iter (internalize f >>> pure iso) (s, x))
+    assert (internalize (fun (x:a) => mkStateT (fun (s:S) => iter (internalize f >>> pure iso) (x, s)))
                        ⩯
                        iter (internalize f >>> pure iso)).
     { repeat red.
-      destruct a2.
+      destruct a1.
       unfold internalize.
-      cbn.  reflexivity.
+      cbn. reflexivity.
     }
    apply H.
    reflexivity.
@@ -317,7 +315,7 @@ Section State.
    rewrite internalize_cat.
    (* SAZ This proof can probably use less unfolding *)
    repeat red.
-   destruct a2.
+   destruct a1.
    unfold cat, Cat_Kleisli. cbn.
    repeat rewrite bind_bind.
    unfold internalize, pure.
@@ -325,7 +323,7 @@ Section State.
    apply Proper_bind.
     - reflexivity.
     - repeat red.
-      destruct a3 as [s' [x | [y | z]]].
+      destruct a2 as [[x | [y | z]] s'].
       + rewrite bind_ret_l.
         cbn. unfold id_, Id_Kleisli, pure.
         rewrite bind_ret_l.
